LeanGrow/FFI/EETrick.lean
@@ -8,3 +8,5 @@ partial def eeTrickImp (n : Nat) : Nat :=
   if n == 0
   then 1
   else n * (eeTrick (n-1))
+ 
+-- is this affected by https://github.com/leanprover/lean4/pull/12930
