LeanGrow/Src/Data/SetTrie/Theory/Model.lean
@@ -1,0 +1,44 @@
+
+
+import LeanGrow.Src.Data.SetTrie.Operations
+import Mathlib.Data.Finset.Card
+
+open Finset
+
+def StudyST (α : Type) := SetTrie Unit (Finset α)
+
+
+variable {α : Type} [DecidableEq α]
+
+def SetTrie.fold {γ : Type _} (c : SetTrie α β) (init : γ) (merge : γ → β → γ) : γ :=
+  match c with
+  | .root c => c.foldl (fun s t => (SetTrie.fold t s merge)) init
+  | .node q c => merge (c.foldl (fun s t => (SetTrie.fold t s merge)) init) q
+  | .leaf _ => init
+
+
+namespace StudyST
+
+abbrev fold {γ : Type _} (c : StudyST α) (init : γ) (merge : γ → (Finset α) → γ) : γ :=
+  SetTrie.fold c init merge
+
+def univ (st : StudyST α) : Finset α :=
+  st.fold ∅ (fun x y => x ∪ y)
+
+def size (st : StudyST α) : Nat :=
+  st.fold 0 (fun x y => x + y.card)
+
+def allNodes (st : StudyST α) (P : (Finset α) → Prop) : Prop :=
+  st.fold True (fun x y => x ∧ P y)
+
+def someNode (st : StudyST α) (P : (Finset α) → Prop) : Prop :=
+  st.fold True (fun x y => x ∧ P y)
+
+def hasElem (st : StudyST α) (a : α) : Prop :=
+  st.someNode (fun x => a ∈ x)
+
+def hasNode (st : StudyST α) (n : Finset α) : Prop :=
+  st.someNode (fun x => n = x)
+
+def sets (st : StudyST α) : Finset (Finset α) :=
+  st.fold ∅ (fun x y => x.image (fun z => z ∪ y))
