LeanGrow/Src/Data/SetTrie/Theory/ModelProps.lean
@@ -1,0 +1,26 @@
+
+
+import LeanGrow.Src.Data.SetTrie.Theory.Model
+import Mathlib.Data.Finset.Union
+
+
+open Finset
+
+namespace StudyST
+
+variable {α : Type} [DecidableEq α]
+
+#check SetTrie.fold.induct
+
+#check Finset.biUnion
+
+theorem biUnion_sets_univ (st : StudyST α) : st.sets.biUnion id = st.univ := by
+  induction st, () using SetTrie.fold.induct with
+  | case1 _ kids ih_kids =>
+    unfold sets univ fold SetTrie.fold
+    sorry
+  | case2 _ key kids ih_kids =>
+    sorry
+  | case3 _ =>
+    unfold sets univ fold SetTrie.fold
+    rfl
