LeanGrow/Src/Utils/Lean/Proofs/Plausible.lean
@@ -1,0 +1,95 @@
+
+
+import Plausible
+
+import Lean
+
+open Plausible
+
+
+#check Lean.evalConst
+
+#check Lean.Compiler.LCNF.Code
+
+
+#check Lean.IR.Decl
+
+#check Lean.addAndCompile
+
+
+#check Lean.Compiler.LCNF.ToLCNF.toLCNF
+
+
+#check Lean.Compiler.LCNF.compile
+
+def testFun (x : Nat) : Nat :=
+  (x+1) * x
+
+
+open Lean
+
+def test0 (n : Name := `testFun) : CoreM Unit := do
+  let res ← Lean.Compiler.LCNF.compile #[n]
+  IO.println <| toString res[0]!
+
+-- #eval test0
+
+
+def test1 (n : Name := `testFun) : CoreM Unit := do
+  let res ← Lean.Compiler.LCNF.compile #[n]
+  for d in res do
+    IO.println <| toString d
+
+-- #eval test1
+
+
+
+def testinFun (x : Nat) : Nat :=
+  42 + testFun x
+
+-- #eval test1 `testinFun
+
+
+set_option trace.compiler.ir.result false
+
+#check Lean.IR.compile
+
+#check Lean.IR.findEnvDecl
+
+def testIRget (n : Name) : CoreM Unit := do
+  let env ← getEnv
+  let .some de := Lean.IR.findEnvDecl env n | throwError "aahh"
+    IO.println <| toString de
+
+
+#eval testIRget `testinFun
+
+
+
+#exit
+
+
+#check Lean.IR.Expr
+
+#print IR.VarId
+#print IR.Index
+
+structure MemoState where
+  stack : Nat
+  heap : Array (IR.VarId × Nat)
+deriving Inhabited
+
+instance : Repr MemoState where
+  reprPrec s _ := s!"stack {s.stack} heap {s.heap.toList}"
+
+def Lean.IR.Expr.memoWatch (var : IR.VarId) (s : MemoState) : IR.Expr → MemoState
+  | .ctor _ _ => {s with heap := s.heap.push (var, 1)}
+  | .fap _ as | .ap _ as => {s with stack := s.stack + as.size}
+  | _ => s
+
+
+def Lean.IR.FnBody.memoWatch (s : MemoState) : IR.FnBody → MemoState
+  | .vdecl var _ e nx => nx.memoWatch (e.memoWatch var s)
+  | .inc var c _ _ nx =>
+      match s.heap.findIdx? (fun (v,_) => v == var) with
+      | .none => panic! "inc on unknown var ..."
